src/AlgEffectus/Core/TypeSafety.lean
@@ -1,0 +1,191 @@
+import AlgEffectus.Core.Parser
+import AlgEffectus.Core.Semantics
+import AlgEffectus.Core.Substitution
+import AlgEffectus.Core.Typing
+import Std.Data.HashMap
+import Std.Data.HashMap.Lemmas
+import Std.Data.DHashMap.Lemmas
+
+-- import LeanCopilot
+-- import aesop
+
+open AlgEffectus.Core
+open scoped AlgEffectus.Core.Typing
+open scoped AlgEffectus.Core.Semantics
+
+open Std
+lemma insert_insert_eq_override {α β} [BEq α] [Hashable α] (m : Std.HashMap α β) (k : α) (v₁ v₂ : β) :
+  (m.insert k v₁).insert k v₂ = m.insert k v₂ := by
+  sorry
+
+mutual
+  lemma substComp_retC_eq_retC_substValue (x : Name) (vA : Value) (v : Value) :
+      substComp x vA (Computation.retC v) = Computation.retC (substValue x vA v) := by
+    unfold substComp substValue StateT.run
+    simp [substCompM]; rfl
+
+  lemma subst_val_preserves
+      {σ Γ x vA A v B}
+      (hv : σ, Γ ⊢ᵥ vA : A)
+      (hvs: σ, (Γ.insert x A) ⊢ᵥ v : B)
+    : σ, Γ ⊢ᵥ (substValue x vA v) : B := by
+    unfold substValue StateT.run
+    cases v with
+    | varV n => cases hvs with
+      | var h_mem =>
+        simp [substValueM] at *
+        split_ifs with hnx
+        · -- 1.  n = x  ----------------------------------------------------
+          cases hnx
+          have hAB : A = B := by
+            have h': (Γ.insert x A).get? x = some A := by simp
+            simp [h'] at h_mem; exact h_mem
+          cases hAB; simpa using hv
+        · -- 2.  n ≠ x  ----------------------------------------------------
+          have hΓ : Γ.get? n = some B := by
+            simp [hnx]; simp [Std.HashMap.getElem?_insert] at h_mem
+            rwa [if_neg] at h_mem; tauto
+          simpa using TyVal.var hΓ
+    | ttV => cases hvs with
+      | tt => simpa [substValueM] using TyVal.tt
+    | ffV => cases hvs with
+      | ff => simpa [substValueM] using TyVal.ff
+    | funV x c => cases hvs with
+      | fun_ hbody =>
+        rename_i x' A' C
+        simp [substValueM] at *
+        split_ifs with hnx
+        · -- 1.  x = x'  ----------------------------------------------------
+          cases hnx
+          split; rename_i  y result' snd' heq'
+          cases heq'
+          have h₁: σ, Γ ⊢ᵥ (Value.funV x' c) :  (VTy.funT A' C) := by
+            apply TyVal.fun_
+            have h₀: (Γ.insert x' A).insert x' A' = Γ.insert x' A' := by
+              apply insert_insert_eq_override
+            simp [h₀] at hbody; exact hbody
+          exact h₁
+        · -- 2.  x ≠ x'  ----------------------------------------------------
+          rename_i h'
+          cases hbody
+          sorry
+        · -- 3.
+          sorry
+    | handV h =>
+      simp [substValueM] at *
+      cases h with
+      | mk rb rc opcls =>
+        cases hvs
+        sorry
+
+
+        simp [substHandlerM]
+        sorry
+
+
+  lemma subst_comp_preserves
+      {σ Γ x vA A c C}
+      (hv : σ, Γ ⊢ᵥ vA : A)
+      (hc : σ, (Γ.insert x A) ⊢ c : C)
+    : σ, Γ ⊢ (substComp x vA c) : C := by
+    cases c with
+    | retC v =>
+      cases hc with | ret hv_v =>
+      rename_i B Δ
+      admit
+    | callC op arg k body =>
+      admit
+    | seqC x c₁ c₂ => admit
+    | ifC b t e => admit
+    | appC f a => admit
+    | withC h c => admit
+
+  lemma subst_hdl_preserves
+      {σ Γ x vA A h C D}
+      (hv : σ, Γ ⊢ᵥ vA : A)
+      (hh : TyHdl σ (Γ.insert x A) h C D)
+    : TyHdl σ Γ (substHandler x vA h) C D
+    := by admit
+end
+
+theorem preservation {σ Γ c c' C} :
+  (σ, Γ ⊢ c : C) → (c ⤳ c') → (σ, Γ ⊢ c' : C)
+:= by
+  intro hTy hStep
+  induction hStep generalizing C with
+  | seq_step h₁ ih  =>
+    rename_i x c₁ c₁' c₂
+    cases hTy with | seq t₁ t₂ =>
+      rename_i A B Δ
+      have hTy₁' : σ, Γ ⊢ c₁' : (A !{Δ}) := by
+        apply ih; exact t₁
+      have hTy₂' : σ, Γ.insert x A ⊢ c₂ : (B !{Δ}) := by
+        exact t₂
+      apply TyComp.seq hTy₁' hTy₂'
+  | seq_return =>
+    rename_i x v c₁
+    cases hTy with | seq t₁ t₂ =>
+      rename_i A B Δ
+      cases t₁ with | ret t₁' =>
+        exact subst_comp_preserves t₁' t₂
+  | seq_op     => admit
+  | if_true    => admit
+  | if_false   => admit
+  | app_β      => admit
+  | with_step  => admit
+  | with_ret   => admit
+  | with_handled   => admit
+  | with_unhandled => admit
+
+theorem progress {σ c A Δ} :
+  (σ, ∅ ⊢ c : (A !{Δ})) →
+  (∃ v, c = Computation.retC v) ∨
+  (∃ op v k cBody, c = Computation.callC op v k cBody ∧ op ∈ Δ) ∨
+  (∃ c', c ⤳ c')
+:= by
+  intro hTy
+  cases hTy with
+  | ret hVal        => admit
+  | call_ sig targ tcont mem => admit
+  | seq t1 t2       => admit
+  | app tf ta       => admit
+  | if_ tb tt te    => admit
+  | with_ th tc     => admit
+
+-- mutual
+--   lemma weaken_val {σ Γ x A v B} (hv : σ, Γ ⊢ᵥ v : B) :
+--     σ, (Γ.insert x A) ⊢ᵥ v : B := by
+--     cases hv with
+--     | var h_mem =>
+--       rename_i n; apply TyVal.var
+--       simp [Std.HashMap.getElem?_insert]
+--       simp at h_mem
+--       by_cases h_eq_keys : x = n
+--       · rw [← h_eq_keys] at h_mem
+--         sorry
+--       · split <;> simp_all
+--     | tt => exact TyVal.tt
+--     | ff => exact TyVal.ff
+--     | fun_ hbody =>
+--       rename_i x' A' C body; apply TyVal.fun_
+--       by_cases h_eq_keys : x = x'
+--       · sorry
+--       · sorry
+--       rw [hΓ]; apply weaken_comp; exact hbody
+--     | hand h =>
+--       admit
+--
+--
+--   lemma weaken_comp
+--       {σ Γ x A c C}
+--       (hc : TyComp σ Γ c C) :
+--       TyComp σ (Γ.insert x A) c C := by admit
+--
+--   lemma weaken_hdl {σ Γ x A h C D} (hh : TyHdl σ Γ h C D) :
+--     TyHdl σ (Γ.insert x A) h C D := by
+--     cases hh with
+--     | mk hret hops heff =>
+--       rename_i rb rc opcs A' B' Δ Δ'
+--       apply TyHdl.mk
+--       repeat admit
+-- end
